Trace sets are now defined as binary relations.

coq/simple-instance/Shape.v
@@ -21,9 +21,10 @@ Definition get_component_idS (s:shape) :
 
 
 (* _____________________________________ 
-              WELL-FORMEDNESS
+             SOURCE LANGUAGE
    _____________________________________ *)
 
+(* ------- Well-formedness ------- *)
 Inductive wellformed_shape : shape -> Prop :=
   | WF_shape : forall s,
     let Is := get_interfacesS s in
@@ -32,27 +33,21 @@ Inductive wellformed_shape : shape -> Prop :=
     incl comps_id (dom2partial (dom_interfaces Is)) ->
     wellformed_shape s.
 
-(* _____________________________________ 
-                HAS SHAPE
-   _____________________________________ *)
 
+(* ------- Has shape ------- *)
 Reserved Notation "'PROGRAM_SHAPE' P ∈• s" (at level 40).
-Inductive program_has_shape (P:Source.partial_program) :
-  shape -> Prop :=
-  | SH_program : forall s,
-    let Is := get_interfacesS s in
-    let comps_id := get_component_idS s in 
+Inductive program_has_shape :
+  Source.partial_program -> shape -> Prop :=
+  | SH_program : forall P Is comps_id,
     wellformed_partial_program_alt Is P ->
     (compsPartialProgram P = comps_id) ->
-    PROGRAM_SHAPE P ∈• s
+    PROGRAM_SHAPE P ∈• (Is, comps_id)
   where "'PROGRAM_SHAPE' P ∈• s" := (program_has_shape P s).
 
 Reserved Notation "'CONTEXT_SHAPE' P ∈∘ s" (at level 40).
-Inductive context_has_shape (P:Source.partial_program) :
-  shape -> Prop :=
-  | SH_context : forall s,
-    let Is := get_interfacesS s in
-    let comps_id := get_component_idS s in
+Inductive context_has_shape :
+  Source.partial_program -> shape -> Prop :=
+  | SH_context : forall P Is comps_id,
     let f C x :=
       match C with
       | Some C' =>
@@ -70,5 +65,55 @@ Inductive context_has_shape (P:Source.partial_program) :
     wellformed_partial_program_alt Is P ->
     dom_partial_program P = 
       (filter not_in_compsId (dom2partial (compsInterface Is))) ->
-    CONTEXT_SHAPE P ∈∘ s
-  where "'CONTEXT_SHAPE' P ∈∘ s" := (context_has_shape P s). 
+    CONTEXT_SHAPE P ∈∘ (Is, comps_id)
+  where "'CONTEXT_SHAPE' P ∈∘ s" := (context_has_shape P s).
+
+(* ------- Context application ------- *)
+Definition unify_components 
+  (K : option component * option component) : component :=
+  match K with
+  | (Some k1', None) => k1'
+  | (None, Some k2') => k2'
+  | _ => (0,0,[],0,0,[])
+  end.
+
+Definition context_application (A P : Source.partial_program) :
+  Source.program :=
+  map unify_components (combine A P).
+
+
+(* _____________________________________ 
+                  PROOFS
+   _____________________________________ *)
+
+Theorem context_application_preserves_wellformedness :
+  forall A P s, 
+  (wellformed_shape s) /\ 
+  (CONTEXT_SHAPE A ∈∘ s) /\ (PROGRAM_SHAPE P ∈• s) ->
+  wellformed_whole_program (context_application A P).
+Proof.
+Admitted.
+
+
+(* _____________________________________ 
+             TARGET LANGUAGE
+   _____________________________________ *)
+
+(* ------- Has shape ------- *)
+
+Reserved Notation "'LL_PROGRAM_SHAPE' P ∈• s" (at level 40).
+Inductive ll_program_has_shape : 
+  Target.program -> shape -> Prop :=
+  | SH_LLprogram : forall Is_p mem E Is comps_id,
+    (forall i, (In i Is_p) -> 
+      ((nth (get_name i) Is (0,0,[])) = i)) ->
+    (dom_entry_points E = dom_global_memory mem) ->
+    (dom_global_memory mem = 
+      (dom2partial (compsInterface Is_p))) ->
+    (dom2partial (compsInterface Is_p) = comps_id) ->
+    LL_PROGRAM_SHAPE (Is_p, mem, E) ∈• (Is, comps_id)
+  where "'LL_PROGRAM_SHAPE' P ∈• s" := 
+  (ll_program_has_shape P s).
+
+(* TODO *)
+
